src/ManCompSoundness.v
@@ -1,0 +1,114 @@
+Require Import Manifest Manifest_Compiler Manifest_Generator 
+  Maps Term_Defs List Cvm_St Cvm_Impl ErrorStMonad_Coq StructTactics Cvm_Monad EqClass Manifest_Admits.
+
+Require Import Auto.
+
+Lemma map_get_minify : forall {A B : Type} `{EqClass A} `{EqClass B} (m : MapC A B) (a : A) b l,
+  map_get m a = Some b ->
+  (map_get 
+    (minify_mapC 
+      m 
+      (fun x => if (in_dec (EqClass_impl_DecEq _) x (a :: l)) then true else false))
+    a) = Some b.
+Proof.
+  induction m; simpl in *; intuition; eauto;
+  repeat (break_match; simpl in *; eauto).
+  - destruct o; subst; find_inversion; try congruence.
+  - destruct f; left; rewrite eqb_leibniz in Heqb0; eauto.
+Qed.
+
+
+
+(* map_get (minify_mapD Local_Plcs (fun _ : Plc => false)) p1 *)
+
+Definition lib_supports_manifest (al : AM_Library) (am : Manifest) : Prop :=
+  (forall (a : ASP_ID), In a am.(asps) -> exists cb, Maps.map_get al.(Local_ASPS) a = Some cb) /\
+  (forall (up : Plc), In up am.(uuidPlcs) -> exists b, Maps.map_get al.(Local_Plcs) up = Some b) /\
+  (forall (pkp : Plc), In pkp am.(pubKeyPlcs) -> exists b, Maps.map_get al.(Local_PubKeys) pkp = Some b).
+
+Ltac unfolds :=
+  repeat monad_unfold;
+  repeat unfold manifest_compiler, generate_ASP_dispatcher, 
+    generate_Plc_dispatcher, generate_PubKey_dispatcher,
+    generate_UUID_dispatcher, lib_supports_manifest in *;
+  simpl in *; 
+  repeat (match goal with
+      | x : cvm_st |- _ => destruct x
+      | x : AM_Config |- _ => destruct x
+      | x : AM_Library |- _ => destruct x
+      | x : CallBackErrors |- _ => destruct x
+  end; simpl in *; eauto);
+  intuition.
+
+Theorem manifest_compiler_sound : forall t p envM,
+  manifest_generator t p = envM ->
+  (forall p' absMan, 
+    map_get envM p' = Some absMan ->
+    (forall amLib amConf, 
+      lib_supports_manifest amLib absMan ->
+      manifest_compiler absMan amLib = amConf ->
+      (forall st,
+        st.(st_AM_config) = amConf ->
+        exists st', 
+          build_cvm (copland_compile t) st = (resultC tt, st') \/
+          build_cvm (copland_compile t) st = (errC (dispatch_error Runtime), st')
+      )
+    )
+  )
+  .
+Proof.
+  induction t; simpl in *; intros.
+  - destruct a; simpl in *; repeat (ff; simpl in *; eauto); unfolds;
+    invc H3.
+    * destruct (H a0); intuition;
+      eapply map_get_minify with (l := nil) in H0; simpl in *.
+      break_match; setoid_rewrite H0 in Heqo; invc Heqo;
+      repeat break_match; intuition; eauto;
+      invc Heqr2; eauto.
+    * destruct (H a0); intuition;
+      eapply map_get_minify with (l := nil) in H0; simpl in *.
+      break_match; setoid_rewrite H0 in Heqo; invc Heqo;
+      repeat break_match; intuition; eauto;
+      invc Heqr2; eauto.
+    * destruct (H sig_aspid); intuition;
+      eapply map_get_minify with (l := nil) in H0; simpl in *.
+      break_match; setoid_rewrite H0 in Heqo; invc Heqo;
+      repeat break_match; intuition; eauto;
+      invc Heqr2; eauto.
+    * destruct (H hsh_aspid); intuition;
+      eapply map_get_minify with (l := nil) in H0; simpl in *.
+      repeat break_match. setoid_rewrite H0 in Heqr2; invc Heqo;
+      repeat break_match; intuition; eauto;
+      invc Heqr2; eauto.
+      rewrite H0 in Heqo.
+    * repeat monad_unfold;
+  repeat unfold manifest_compiler, generate_ASP_dispatcher, 
+    generate_Plc_dispatcher, generate_PubKey_dispatcher,
+    generate_UUID_dispatcher, lib_supports_manifest in *;
+  simpl in *; repeat break_match; try solve_by_inversion; 
+    cbn in *; unfold runErr in *; simpl in *;
+      repeat (monad_unfold; cbn in *; find_inversion);
+      monad_unfold;
+      repeat dunit;
+      unfold snd in *; intuition; eauto.
+      
+      
+       destruct par.
+      break_let.
+    try (destruct (H a0); intuition; eauto).
+    * eapply map_get_minify in H3. 
+       
+      erewrite H0 in Heqo.
+    * unfold manifest_compiler
+    * 
+      unfold manifest_compiler in H3; simpl in *; ff; simpl in *; eauto. ff.
+      | H1 : build_cvm t1 _ = (_, _), H2 : build_cvm t1 _ = (_, _) |- _ =>
+        eapply IHt1 in H1; eauto; simpl in *; intuition; subst; try congruence; eauto
+      | H1 : build_cvm t2 _ = (_, _), H2 : build_cvm t2 _ = (_, _) |- _ =>
+        eapply IHt2 in H1; eauto; simpl in *; intuition; subst; try congruence; eauto
+      end.
+      destruct st; simpl in *; repeat (ff; simpl in *; eauto).
+    * 
+
+  
+Qed.
